Rename some lemmas under a namespace

CBPV/Evaluation.lean
@@ -2,14 +2,14 @@ import CBPV.Syntax
 
 open Val Com
 
-/-*----------------------
-  Single-step reduction
-----------------------*-/
+/-*-----------------------
+  Single-step evaluation
+-----------------------*-/
 
 section
 set_option hygiene false
-local infix:40 "⇒" => Step
-inductive Step : Com → Com → Prop where
+local infix:40 "⇒" => Eval
+inductive Eval : Com → Com → Prop where
   | force {m} : force (thunk m) ⇒ m
   | lam {m v} : app (lam m) v ⇒ m⦃v⦄
   | ret {v m} : letin (ret v) m ⇒ m⦃v⦄
@@ -24,10 +24,10 @@ inductive Step : Com → Com → Prop where
     ----------------------
     letin m n ⇒ letin m' n
 end
-infix:40 "⇒" => Step
+infix:40 "⇒" => Eval
 
--- Single-step reduction is deterministic
-theorem stepDet {m n₁ n₂} (r₁ : m ⇒ n₁) (r₂ : m ⇒ n₂) : n₁ = n₂ := by
+-- Single-step evaluation is deterministic
+theorem evalDet {m n₁ n₂} (r₁ : m ⇒ n₁) (r₂ : m ⇒ n₂) : n₁ = n₂ := by
   induction r₁ generalizing n₂
   all_goals cases r₂; try rfl
   all_goals apply_rules [appCong, letinCong]
@@ -39,27 +39,27 @@ theorem stepDet {m n₁ n₂} (r₁ : m ⇒ n₁) (r₂ : m ⇒ n₂) : n₁ = n
 
 section
 set_option hygiene false
-local infix:40 "⇒⋆" => Steps
-inductive Steps : Com → Com → Prop where
+local infix:40 "⇒⋆" => Evals
+inductive Evals : Com → Com → Prop where
   | refl a : a ⇒⋆ a
   | trans {a b c} : a ⇒ b → b ⇒⋆ c → a ⇒⋆ c
 end
-infix:40 "⇒⋆" => Steps
-open Steps
+infix:40 "⇒⋆" => Evals
+open Evals
 
-theorem stepSteps {a b} (r : a ⇒ b) : a ⇒⋆ b := .trans r (.refl b)
+theorem Evals.once {a b} (r : a ⇒ b) : a ⇒⋆ b := .trans r (.refl b)
 
-theorem trans' {a b c} (r₁ : a ⇒⋆ b) (r₂ : b ⇒⋆ c) : a ⇒⋆ c := by
+theorem Evals.trans' {a b c} (r₁ : a ⇒⋆ b) (r₂ : b ⇒⋆ c) : a ⇒⋆ c := by
   induction r₁ generalizing c
   case refl => exact r₂
   case trans r₁ _ ih => exact .trans r₁ (ih r₂)
 
-theorem stepsApp {m n v} (r : m ⇒⋆ n) : app m v ⇒⋆ app n v := by
+theorem Evals.app {m n v} (r : m ⇒⋆ n) : app m v ⇒⋆ app n v := by
   induction r
   case refl => exact .refl _
   case trans r _ ih => exact .trans (.app r) ih
 
-theorem stepsLet {m m' n} (r : m ⇒⋆ m') : letin m n ⇒⋆ letin m' n := by
+theorem Evals.let {m m' n} (r : m ⇒⋆ m') : letin m n ⇒⋆ letin m' n := by
   induction r
   case refl => exact .refl _
   case trans r _ ih => exact .trans (.letin r) ih
@@ -71,7 +71,7 @@ theorem confluence {m n₁ n₂} (r₁ : m ⇒⋆ n₁) (r₂ : m ⇒⋆ n₂) :
   case trans r₁ rs₁ ih =>
     cases r₂
     case refl => exact ⟨_, refl _, trans r₁ rs₁⟩
-    case trans r₂ rs₂ => rw [stepDet r₁ r₂] at *; exact ih rs₂
+    case trans r₂ rs₂ => rw [evalDet r₁ r₂] at *; exact ih rs₂
 
 /-*----------------------------
   Normal forms and evaluation
@@ -80,14 +80,14 @@ theorem confluence {m n₁ n₂} (r₁ : m ⇒⋆ n₁) (r₂ : m ⇒⋆ n₂) :
 @[simp]
 def nf : Com → Prop
   | lam _ | ret _ => True
-  | force _ | app _ _ | letin _ _ | case _ _ _ => False
+  | force _ | .app _ _ | letin _ _ | case _ _ _ => False
 
 theorem nfStepn't {m n} (nfm : nf m) : ¬ m ⇒ n := by
   cases m <;> simp at *
   all_goals intro r; cases r
 
-def Eval (m n : Com) := m ⇒⋆ n ∧ nf n
-infix:40 "⇓" => Eval
+def Norm (m n : Com) := m ⇒⋆ n ∧ nf n
+infix:40 "⇓" => Norm
 
 /-*---------------------
   Strong normalization
@@ -96,10 +96,10 @@ infix:40 "⇓" => Eval
 inductive SN : Com → Prop where
   | sn : ∀ m, (∀ n, m ⇒ n → SN n) → SN m
 
-theorem nfSN {m} (nfm : nf m) : SN m := by
+theorem SN.nf {m} (nfm : nf m) : SN m := by
   constructor; intro n r; cases nfStepn't nfm r
 
-theorem stepsSN {m n} (r : m ⇒⋆ n) (nfn : nf n) : SN m := by
+theorem Evals.sn {m n} (r : m ⇒⋆ n) (nfn : nf n) : SN m := by
   induction r
-  case refl => exact nfSN nfn
-  case trans r _ ih => constructor; intro _ r'; rw [← stepDet r r']; exact ih nfn
+  case refl => exact .nf nfn
+  case trans r _ ih => constructor; intro _ r'; rw [← evalDet r r']; exact ih nfn
